theories/Concatenation.v
@@ -1,0 +1,100 @@
+From LambdaST Require Import
+  Derivative
+  Invert
+  Prefix
+  Types.
+
+(* Definition B.20 *)
+Inductive PfxCat : prefix -> prefix -> prefix -> Prop :=
+  | PfxCatEpsEmp :
+      PfxCat PfxEpsEmp PfxEpsEmp PfxEpsEmp
+  | PfxCatOneEmp : forall p,
+      PfxTyped p 1 ->
+      PfxCat PfxOneEmp p p
+  | PfxCatOneFull :
+      PfxCat PfxOneFull PfxEpsEmp PfxOneFull
+  | PfxCatParPair : forall p1 p1' p1'' p2 p2' p2'',
+      PfxCat p1 p1' p1'' ->
+      PfxCat p2 p2' p2'' ->
+      PfxCat (PfxParPair p1 p2) (PfxParPair p1' p2') (PfxParPair p1'' p2'')
+  | PfxCatCatFst : forall p p' p'',
+      PfxCat p p' p'' ->
+      PfxCat (PfxCatFst p) (PfxCatFst p') (PfxCatFst p'')
+  | PfxCatCatFstCatBoth : forall p p' p'' p''',
+      PfxCat p p' p'' ->
+      PfxCat (PfxCatFst p) (PfxCatBoth p' p''') (PfxCatBoth p'' p''')
+  | PfxCatCatBoth : forall p p' p'' p''',
+      PfxCat p' p'' p''' ->
+      PfxCat (PfxCatBoth p p') p'' (PfxCatBoth p p''')
+  | PfxCatSumEmp : forall p,
+      PfxCat PfxSumEmp p p
+  | PfxCatSumInl : forall p p' p'',
+      PfxCat p' p'' p'' ->
+      PfxCat (PfxSumInl p) p' (PfxSumInl p'')
+  | PfxCatSumInr : forall p p' p'',
+      PfxCat p p' p'' ->
+      PfxCat (PfxSumInr p) p' (PfxSumInr p'')
+  | PfxCatStarEmp : forall p,
+      PfxCat PfxStarEmp p p
+  | PfxCatStarDone :
+      PfxCat PfxStarDone PfxEpsEmp PfxStarDone
+  | PfxCatStarFirst : forall p p' p'',
+      PfxCat p p' p'' ->
+      PfxCat (PfxStarFirst p) (PfxCatFst p') (PfxStarFirst p'')
+  | PfxCatStarFirstStarRest : forall p p' p'' p''',
+      PfxCat p p' p'' ->
+      PfxCat (PfxStarFirst p) (PfxCatBoth p' p''') (PfxStarRest p'' p''')
+  | PfxCatStarRest : forall p p' p'' p''',
+      PfxCat p' p'' p''' ->
+      PfxCat (PfxStarRest p p') p'' (PfxStarRest p p''')
+  .
+
+(* TODO: Either something is wrong with the definition of concatenation for inl or this is just difficult *)
+Lemma pfx_cat_inl_unsure : forall p' p''1 p''2,
+  PfxCat p' p''1 p''1 ->
+   (forall p''2, PfxCat p' p''1 p''2 -> p''1 = p''2) ->
+   PfxCat p' p''2 p''2 ->
+   PfxSumInl p''1 = PfxSumInl p''2.
+Proof.
+  intros p' p''1 p''2 H1 IH H2. f_equal. Abort.
+
+(* Theorem B.21, part I *)
+Theorem prefix_concat_unique : forall p p' p''1 p''2,
+  PfxCat p p' p''1 ->
+  PfxCat p p' p''2 ->
+  p''1 = p''2.
+Proof.
+  intros p p' p''1 p''2 H1 H2. generalize dependent p''2. induction H1; intros;
+  invert H2;
+  try apply IHPfxCat in H3;
+  try apply IHPfxCat in H5;
+  try apply IHPfxCat in H0;
+  subst; try reflexivity.
+  - apply IHPfxCat1 in H5. apply IHPfxCat2 in H6. subst. reflexivity.
+  - Abort. (* apply (pfx_cat_inl_unsure p'); assumption. *)
+
+(* Theorem B.21, part II *)
+Theorem prefix_concat_exists_when_typed : forall p p' s dps ,
+  PfxTyped p s ->
+  Derivative p s dps ->
+  PfxTyped p' dps ->
+  exists p'' dp'dps,
+    Derivative p' dps dp'dps /\
+    PfxCat p p' p'' /\
+    PfxTyped p'' s /\
+    Derivative p'' s dp'dps.
+Proof.
+  intros p p' s dps Ht Hd Ht'. generalize dependent p'. generalize dependent Ht.
+  induction Hd; intros; invert Ht.
+  - invert Ht'; repeat eexists; repeat constructor.
+  - invert Ht'; repeat eexists; repeat constructor.
+  - invert Ht'; repeat eexists; repeat constructor.
+  - invert Ht'. specialize (IHHd1 H2). specialize (IHHd2 H4).
+    apply IHHd1 in H3 as [p''1 [dp'dps1 [H21 [H22 [H23 H24]]]]].
+    apply IHHd2 in H5 as [p''2 [dp'dps2 [H31 [H32 [H33 H34]]]]].
+    repeat eexists; repeat constructor;
+    try apply H21; try apply H31; try apply H22; try apply H32; assumption.
+  - specialize (IHHd H1). invert Ht';
+    apply IHHd in H2 as [p'' [dp'dps [h1 [h2 [h3 h4]]]]].
+    + repeat eexists; repeat constructor; [apply h1 | apply h2 | |]; assumption.
+    + repeat eexists; repeat constructor; try assumption. Abort.
