theories/Hole.v
@@ -1,0 +1,44 @@
+From LambdaST Require Import
+  Context.
+
+Inductive hole : Set :=
+  | HoleHere
+  | HoleCommaL (lhs : hole) (rhs : context)
+  | HoleCommaR (lhs : context) (rhs : hole)
+  | HoleSemicL (lhs : hole) (rhs : context)
+  | HoleSemicR (lhs : context) (rhs : hole)
+  .
+
+Fixpoint fill h y :=
+  match h with
+  | HoleHere => y
+  | HoleCommaL lhs rhs => CtxComma (fill lhs y) rhs
+  | HoleCommaR lhs rhs => CtxComma lhs (fill rhs y)
+  | HoleSemicL lhs rhs => CtxSemic (fill lhs y) rhs
+  | HoleSemicR lhs rhs => CtxSemic lhs (fill rhs y)
+  end.
+
+Inductive FillWith y : hole -> context -> Prop :=
+  | FillHere :
+      FillWith y HoleHere y
+  | FillCommaL : forall lhs rhs lhs',
+      FillWith y lhs lhs' ->
+      FillWith y (HoleCommaL lhs rhs) (CtxComma lhs' rhs)
+  | FillCommaR : forall lhs rhs rhs',
+      FillWith y rhs rhs' ->
+      FillWith y (HoleCommaR lhs rhs) (CtxComma lhs rhs')
+  | FillSemicL : forall lhs rhs lhs',
+      FillWith y lhs lhs' ->
+      FillWith y (HoleSemicL lhs rhs) (CtxSemic lhs' rhs)
+  | FillSemicR : forall lhs rhs rhs',
+      FillWith y rhs rhs' ->
+      FillWith y (HoleSemicR lhs rhs) (CtxSemic lhs rhs')
+  .
+
+Theorem reflect_fill : forall h y c,
+  c = fill h y <-> FillWith y h c.
+Proof.
+  split; intros.
+  - subst. generalize dependent y. induction h; intros; simpl in *; constructor; apply IHh.
+  - induction H; simpl; try rewrite IHFillWith; reflexivity.
+Qed.
