theories/Typing.v
@@ -7,6 +7,7 @@ Declare Scope typing_scope.
 
 Reserved Notation "G '|-' x '\in' T" (at level 98).
 
+(*
 Inductive Typed : context -> term -> type -> Prop :=
   | T_Par_R : forall G e1 e2 s t,
       G |- e1 \in s ->
@@ -41,3 +42,4 @@ Inductive Typed : context -> term -> type -> Prop :=
       Gxs |- e' \in t ->
       GD |- TmLet x e e' \in t
 where "G '|-' x '\in' T" := (Typed G x T).
+*)
