Makefile
@@ -6,18 +6,16 @@ SRCDIR:=theories
 SOURCES:=$(shell find $(SRCDIR) -name '*.v')
 MCOQ:=Makefile.coq
 
-all: $(MCOQ)
+all install: $(MCOQ)
 	+$(MAKE) -f $< $@
 
 clean: $(MCOQ)
 	+$(MAKE) -f $< cleanall
 	rm -f _CoqProject .filestoinstall Makefile.coq Makefile.coq.conf result
-	find . -name '*.aux' -o -name '*.glob' -o -name '*.swp' -o -name '*.vo' -o -name '*.vok' -o -name '*.vos' | xargs rm
+	find . -name '*.aux' -o -name '*.glob' -o -name '*.swp' -o -name '*.vo' -o -name '*.vok' -o -name '*.vos' | xargs -r rm
 
 $(MCOQ): _CoqProject
 	$(COQBIN)coq_makefile -f $< -o $@ $(SOURCES)
 
 _CoqProject: $(SRCDIR) Makefile
 	echo '-Q $(SRCDIR) LambdaST' > $@
-
-install: ;
